logging a partial solution for the secure state handler issue in the git log

theories/Secure/SecurityImp/SecurityImpHandler.v
@@ -240,21 +240,160 @@ Definition state_eqit_secure {R1 R2 : Type} (b1 b2 : bool) (RR : R1 -> R2 -> Pro
   forall s1 s2, RS s1 s2 -> eqit_secure Label priv2 (product_rel RS RR) b1 b2 l (m1 s1) (m2 s2).
 
 Definition top2 {R1 R2} (r1 : R1) (r2 : R2) : Prop := True.
+  
 
-Inductive terminates {A} (s1 : S) (P : E2 A -> Prop) : itree E2 (S * A) -> Prop :=
-| terminates_ret : forall r (s2 : S), RS s1 s2 -> terminates s1 P (Ret (s2, r))
-| terminates_tau : forall t, terminates s1 P t -> terminates s1 P (Tau t)
-| terminates_vis : forall (e : E2 A) k, (forall v, terminates s1 P (k v)) -> P e -> terminates s1 P (Vis e k)
+Definition secure_in_nonempty_context {R} (m : stateT S (itree E2) R) :=
+   forall r' : R, state_eqit_secure true true top2 m (ret r').
+
+Definition secure_in_empty_context  {R} (m : stateT S (itree E2) R) :=
+   state_eqit_secure true true (@top2 R R) m (fun s => ITree.spin).
+
+Inductive terminates (s1 : S) (P : forall A, E2 A -> Prop) : forall {A : Type}, itree E2 (S * A) -> Prop :=
+| terminates_ret {R : Type} : forall (r : R) (s2 : S), RS s1 s2 -> terminates s1 P (Ret (s2, r))
+| terminates_tau : forall A (t : itree E2 (S * A)) , terminates s1 P t -> terminates s1 P (Tau t)
+| terminates_vis {A R : Type} : forall (e : E2 A) (k : A -> itree E2 (S * R)) , (forall v, terminates s1 P (k v)) -> P A e -> terminates s1 P (Vis e k)
 .
+
+Instance proper_terminate {R s} {P : forall A, E2 A -> Prop} : Proper (eq_itree (@eq (S *R )) ==> iff) (terminates s P).
+Proof.
+  red. intros t1 t2 Heq. apply Eq.EqAxiom.bisimulation_is_eq in Heq. subst; tauto.
+Qed.
+  
+
 
 Variant handler_respects_priv (A : Type) (e : E1 A) : Prop :=
 | respect_private (SECCHECK : ~ leq (priv1 _ e) l)
-                  (FINCHECK : forall s, terminates s (fun e => ~ leq (priv2 _ e) l) (handler A e s))
+                  (FINCHECK : forall s, terminates s (fun _ e => ~ leq (priv2 _ e) l) (handler A e s))
 | respect_public (SECCHECK : leq (priv1 _ e) l)
                  (RESCHECK : state_eqit_secure true true eq (handler A e) (handler A e))
 .
 
-Context (Hhandler : forall A (e : E1 A), handler_respects_priv A e).
+Variant handler_respects_priv' (A : Type) (e : E1 A) : Prop :=
+| respect_private_ne (SECCHECK : ~ leq (priv1 _ e) l) (SIZECHECK : nonempty A)
+                  (FINCHECK : secure_in_nonempty_context (handler A e) )
+| respect_private_e (SECCHECK : ~ leq (priv1 _ e) l) (SIZECHECK : empty A)
+                  (FINCHECK : secure_in_empty_context (handler A e) )
+| respect_public' (SECCHECK : leq (priv1 _ e) l)
+                 (RESCHECK : state_eqit_secure true true eq (handler A e) (handler A e))
+.
+(*
+Lemma handler_respects_priv_equiv : forall A (e : E1 A) ,
+    nonempty A -> ~ leq (priv1 _ e) l -> (forall s, terminates s (fun _ e => ~ leq (priv2 _ e) l) (handler A e s) ) -> secure_in_nonempty_context (handler A e) .
+Proof.
+  intros A e Hne HCHECK Hsec. destruct RS_PER.
+  do 2 red. intros r s1 s2 Hs. specialize (Hsec s1).
+  induction Hsec.
+  - pfold. constructor. split; try constructor. cbn. eapply PER_Transitive; eauto.
+  - pfold. constructor; auto. pstep_reverse. eapply IHHsec; eauto.
+  - (*no this does not hold*)
+
+
+  intros A e. destruct RS_PER. intros Hsec; destruct Hsec.
+ (* - destruct (classic_empty A).
+    + apply respect_private_e; auto.
+      do 2 red. intros. specialize (FINCHECK s1).
+      remember (handler A e s1) as hes. clear Heqhes.
+      hinduction FINCHECK before RS; intros; subst.
+      * contra_size.
+      * pfold; constructor; auto. pstep_reverse.
+        eapply IHFINCHECK; eauto.
+      * destruct (classic_empty A).
+        -- pcofix CIH. pfold. red. cbn. unpriv_halt.
+        -- pfold. red. cbn. unpriv_co. left. eapply H0; eauto.
+    + apply respect_private_ne; auto. do 2 red. intros.
+      specialize (FINCHECK s1). admit.
+      (* remember (handler A e s1) as hes. 
+      hinduction FINCHECK before RS; intros; subst.
+      * pfold. constructor. split; try constructor. cbn.
+        eapply PER_Transitive; eauto.
+      * pfold. constructor; auto. pstep_reverse. eapply IHFINCHECK; eauto.
+      * pfold. red. cbn. setoid_rewrite itree_eta' at 2. unpriv_ind. *) *)
+   - red in FINCHECK. inv SIZECHECK. specialize (FINCHECK a).
+     apply respect_private; auto. intros. 
+    specialize (FINCHECK s s). 
+    assert (RS s s). admit. (* maybe need that RS is an equiv for this*)
+    specialize (FINCHECK H). cbn in FINCHECK.
+    punfold FINCHECK. red in FINCHECK. cbn in FINCHECK. remember (RetF (s,a) ) as or.
+    remember (handler A e) as m. clear Heqm.
+    remember (observe (m s)) as oms.
+    hinduction FINCHECK before l; intros; try discriminate.
+    + destruct H. destruct r1. destruct r2. cbn in *. use_simpobs.
+      injection Heqor; intros; subst. rewrite Heqoms. constructor.
+      apply PER_Symmetric. auto.
+    + use_simpobs. rewrite Heqoms. constructor.
+      remember (fun s : S => t1) as m'.
+      assert (m' s = t1). subst; auto. rewrite <- H0.
+      eapply IHFINCHECK; eauto. subst; auto.
+    + use_simpobs. rewrite Heqoms. constructor.
+      intros. remember (fun s : S => k1 v) as m'.
+      assert (m' s = k1 v). subst; auto. rewrite <- H2.
+      eapply H0; eauto. subst. auto. auto.
+   - apply respect_private; auto. intros. red in FINCHECK.
+     red in FINCHECK.
+
+
+     red in FINCHECK. apply respect_private; auto. inv SIZECHECK.
+     specialize (FINCHECK a). red in FINCHECK. intros.
+     specialize (FINCHECK s s).
+     assert (RS s s). admit.
+     specialize (FINCHECK H). cbn in FINCHECK. punfold FINCHECK. red in FINCHECK. 
+     cbn in FINCHECK. remember (RetF (s,a)) as or.
+     induction FINCHECK; try discriminate.
+     remember (handler A e s) as hes.
+     induction FINCHECK; try discriminate.
+     + subst.
+      hinduction FINCHECK before E1; intros; subst; try discriminate.
+     +
+
+     admit.
+   - admit.
+   - apply respect_public; auto.
+    
+*)
+(*
+Lemma secure_in_context_terminates_init : forall R (m : stateT S (itree E2 ) R ),
+  (forall s, terminates s (fun _ e => ~ leq (priv2 _ e) l) (m s) ) <-> (secure_in_nonempty_context m \/ secure_in_empty_context m).
+Proof.
+  intros R m. destruct RS_PER. split; intros Hsec.
+  - unfold secure_in_empty_context, secure_in_nonempty_context, state_eqit_secure.
+    enough (forall (s1 s2 : S), RS s1 s2 -> (forall r' : R ,eqit_secure Label priv2 (product_rel RS top2)
+     true true l (m s1) (Ret(s2, r') )) \/ (eqit_secure Label priv2 (product_rel RS (@top2 R R)) true true l (m s1) ITree.spin)).
+    { 
+
+    intros. specialize (Hsec s1).
+    induction Hsec.
+    + cbn. pfold. constructor. split; cbn; auto.
+      * eapply PER_Transitive; eauto.
+      * constructor.
+    + cbn. pfold. constructor; auto. pstep_reverse.
+      apply IHHsec; auto.
+    + pfold. red. cbn.
+      destruct (classic_empty A).
+      * admit. (* need an extra case *)
+      * setoid_rewrite itree_eta' at 2. unpriv_ind. pstep_reverse. eapply H1; eauto.
+      Print Ltac unpriv_ind.
+  - red in Hsec. destruct Hsec as [r' Hsec]. red in Hsec. intros s.
+    specialize (Hsec s s). 
+    assert (RS s s). admit. (* maybe need that RS is an equiv for this*)
+    specialize (Hsec H). cbn in Hsec.
+    punfold Hsec. red in Hsec. cbn in Hsec. remember (RetF (s,r') ) as or.
+    remember (observe (m s)) as oms.
+    hinduction Hsec before l; intros; try discriminate.
+    + destruct H. destruct r1. destruct r2. cbn in *. use_simpobs.
+      injection Heqor; intros; subst. rewrite Heqoms. constructor.
+      apply PER_Symmetric. auto.
+    + use_simpobs. rewrite Heqoms. constructor.
+      remember (fun s : S => t1) as m'.
+      assert (m' s = t1). subst; auto. rewrite <- H0.
+      eapply IHHsec; eauto. subst; auto.
+    + use_simpobs. rewrite Heqoms. constructor.
+      intros. remember (fun s : S => k1 v) as m'.
+      assert (m' s = k1 v). subst; auto. rewrite <- H2.
+      eapply H0; eauto. subst. auto. auto.
+*)
+
+
+Context (Hhandler : forall A (e : E1 A), handler_respects_priv' A e).
 
 Lemma secure_eqit_interp_aux_l {R1 R2} (RR : R1 -> R2 -> Prop) A (e : E1 A) (e' : E2 A) t (k : A -> itree E1 R1) k' r :
   ~ leq (priv1 A e) l ->
@@ -272,29 +411,75 @@ Proof.
     pfold. constructor 11; auto.
   - (* inductive private vis *)
     use_simpobs. rewrite H0. rewrite interp_state_vis.
-    specialize (Hhandler _ e0). inversion Hhandler; try contradiction.
-    specialize (FINCHECK s). induction FINCHECK.
-    + rewrite bind_ret_l. pstep. constructor 11; auto. right. apply CIH; auto.
-      simpl. rewrite H in H1. pstep. apply H1.
-    + rewrite bind_tau. pstep. constructor 11; auto.
-    + rewrite bind_vis. pstep. constructor 13; auto.
+    specialize (Hhandler _ e0). inversion Hhandler; try contradiction; try contra_size.
+    red in FINCHECK. inv SIZECHECK0.
+    specialize (FINCHECK a s s). 
+    assert (RS s s) as Hrefl. admit.
+    specialize (FINCHECK Hrefl). punfold FINCHECK.
+    remember (handler A0 e0) as m. clear Heqm. red in FINCHECK.
+    remember (observe (m s) ) as oms. cbn in FINCHECK. remember (RetF (s,a)) as oRet.
+    hinduction FINCHECK before r; intros; subst; try contradiction; try discriminate.
+    + use_simpobs. rewrite Heqoms. rewrite bind_ret_l. pstep. red. cbn. unpriv_halt.
+      right. eapply CIH; eauto. rewrite H0 in H1. pstep. apply H1.
+    + use_simpobs. rewrite Heqoms.
+      rewrite bind_tau. pstep.  red. cbn. unpriv_halt.
+      pclearbot.
+      left. remember (fun s : S => t1) as m'. assert (t1 = m' s). subst; auto.  rewrite H2. eapply IHFINCHECK; eauto. subst; auto.
+    + use_simpobs. rewrite Heqoms. rewrite bind_vis. pstep. constructor 13; auto.
+      left. remember (fun s : S => k1 b) as m'. assert (k1 b = m' s). subst; auto. rewrite H4. eapply H0; eauto.
+      subst; auto.
   - (* coinductive halting tau *) use_simpobs. rewrite H3. rewrite interp_state_tau.
     pclearbot. pfold. constructor 11; auto.
   - (* coinductive halting vis *)
     use_simpobs. rewrite H3. rewrite interp_state_vis.
-    specialize (Hhandler _ e2). inversion Hhandler; try contradiction.
-    specialize (FINCHECK s). induction FINCHECK.
-    + rewrite bind_ret_l. pstep. constructor 11; auto.
-    + rewrite bind_tau. pstep. constructor 11; auto.
-    + rewrite bind_vis. pstep. constructor 13; auto.
+    specialize (Hhandler _ e2). inversion Hhandler; try contradiction; try contra_size.
+    + red in FINCHECK. inv SIZECHECK0. assert (RS s s). admit.  specialize (FINCHECK a s s H).
+      remember (handler B e2) as m. clear Heqm. punfold FINCHECK.
+      red in FINCHECK. cbn in *. remember (observe (m s)) as oms. remember (RetF (s,a)) as oRet.
+      hinduction FINCHECK before r; intros; subst; try contradiction; try discriminate.
+      * use_simpobs. rewrite Heqoms. rewrite bind_ret_l. pstep. constructor 11; auto.
+      * use_simpobs. rewrite Heqoms. rewrite bind_tau. pstep; constructor; auto.
+        pstep_reverse. remember (fun s : S => t1) as m'.  assert (t1 = m' s). subst; auto.
+        rewrite H1. eapply IHFINCHECK; eauto. subst; auto.
+      * use_simpobs. rewrite Heqoms. rewrite bind_vis. pstep. constructor 13; auto.
+        left. remember (fun s : S => k1 b) as m'. assert (k1 b = m' s). subst; auto. rewrite H4. eapply H0; eauto.
+        subst; auto.
+    + red in FINCHECK. inv SIZECHECK0. assert (RS s s). admit.  specialize (FINCHECK s s H1).
+      cbn in *. remember (handler B e2 s) as tspin. clear Heqtspin. clear CIH Heq.
+      generalize dependent tspin. pcofix CIH. intros. punfold FINCHECK.
+      red in FINCHECK. cbn in *. remember (TauF ITree.spin) as ot. remember (observe tspin) as ots.
+      hinduction FINCHECK before r; intros; subst; try discriminate.
+      * use_simpobs. rewrite Heqots. rewrite bind_tau. pfold. constructor 11; auto.
+        right. eapply CIH; eauto. pclearbot. injection Heqot; intros; subst. auto.
+      * use_simpobs. rewrite Heqots. rewrite bind_tau. pstep; constructor; auto.
+        pstep_reverse.
+      * injection Heqot; intros; subst. eapply IHFINCHECK; eauto.
+      * use_simpobs. rewrite Heqots. rewrite bind_vis. pfold. constructor 13; auto.
+        right. pclearbot. eapply CIH; eauto. injection Heqot; intros; subst. apply H2.
+      * use_simpobs. rewrite Heqots. rewrite bind_vis. pfold. red. cbn. rewrite itree_eta' at 1. unpriv_ind. 
+        pstep_reverse.
+      * use_simpobs. rewrite Heqots. rewrite bind_vis. pfold. pclearbot. red. cbn. unpriv_halt. contra_size.
+  
   - (* coinductive halting vis *)
     use_simpobs. rewrite H3. rewrite interp_state_vis.
-    specialize (Hhandler _ e2). inversion Hhandler; try contradiction.
-    specialize (FINCHECK s). induction FINCHECK.
-    + inversion SIZECHECK. contradiction.
-    + rewrite bind_tau. pstep. constructor 11; auto.
-    + rewrite bind_vis. pstep. constructor 13; auto.
-Qed.
+    specialize (Hhandler _ e2). inversion Hhandler; try contradiction; try contra_size.
+    + red in FINCHECK. inv SIZECHECK0. assert (RS s s). admit.  specialize (FINCHECK s s H1).
+      cbn in *. remember (handler B e2 s) as tspin. clear Heqtspin. clear CIH Heq.
+      generalize dependent tspin. pcofix CIH. intros. punfold FINCHECK.
+      red in FINCHECK. cbn in *. remember (TauF ITree.spin) as ot. remember (observe tspin) as ots.
+      hinduction FINCHECK before r; intros; subst; try discriminate.
+      * use_simpobs. rewrite Heqots. rewrite bind_tau. pfold. constructor 11; auto.
+        right. eapply CIH; eauto. pclearbot. injection Heqot; intros; subst. auto.
+      * use_simpobs. rewrite Heqots. rewrite bind_tau. pstep; constructor; auto.
+        pstep_reverse.
+      * injection Heqot; intros; subst. eapply IHFINCHECK; eauto.
+      * use_simpobs. rewrite Heqots. rewrite bind_vis. pfold. constructor 13; auto.
+        right. pclearbot. eapply CIH; eauto. injection Heqot; intros; subst. apply H2.
+      * use_simpobs. rewrite Heqots. rewrite bind_vis. pfold. red. cbn. rewrite itree_eta' at 1. unpriv_ind. 
+        pstep_reverse.
+      * use_simpobs. rewrite Heqots. rewrite bind_vis. pfold. pclearbot. red. cbn. unpriv_halt. contra_size.
+    
+Admitted.
 
 Lemma secure_eqit_interp_aux_r {R1 R2} (RR : R1 -> R2 -> Prop) A (e : E1 A) (e' : E2 A) t (k : A -> itree E1 R2) k' r :
   ~ leq (priv1 A e) l ->
@@ -312,29 +497,79 @@ Proof.
     pfold. constructor 12; auto.
   - (* inductive private vis *)
     use_simpobs. rewrite H. rewrite interp_state_vis.
-    specialize (Hhandler _ e0). inversion Hhandler; try contradiction.
-    specialize (FINCHECK s). induction FINCHECK.
-    + rewrite bind_ret_l. pstep. constructor 12; auto. right. apply CIH; auto.
-      simpl. rewrite H0 in H1. pstep. apply H1.
-    + rewrite bind_tau. pstep. constructor 12; auto.
-    + rewrite bind_vis. pstep. constructor 14; auto.
+    specialize (Hhandler _ e0). inversion Hhandler; try contradiction; try contra_size.
+    red in FINCHECK. inv SIZECHECK0.
+    specialize (FINCHECK a s s). 
+    assert (RS s s) as Hrefl. admit.
+    specialize (FINCHECK Hrefl). punfold FINCHECK.
+    remember (handler A0 e0) as m. clear Heqm. red in FINCHECK.
+    remember (observe (m s) ) as oms. cbn in FINCHECK. remember (RetF (s,a)) as oRet.
+    hinduction FINCHECK before r; intros; subst; try contradiction; try discriminate.
+    + use_simpobs. rewrite Heqoms. rewrite bind_ret_l. pstep. red. cbn. unpriv_halt.
+      right. eapply CIH; eauto. rewrite H2 in H1. pstep. apply H1.
+    + use_simpobs. rewrite Heqoms.
+      rewrite bind_tau. pstep.  red. cbn. unpriv_halt.
+      pclearbot.
+      left. remember (fun s : S => t1) as m'. assert (t1 = m' s). subst; auto.  rewrite H2. eapply IHFINCHECK; eauto. subst; auto.
+    + use_simpobs. rewrite Heqoms. rewrite bind_vis. pstep. constructor 14; auto.
+      left. remember (fun s : S => k1 a0) as m'. assert (k1 a0 = m' s). subst; auto. rewrite H4. eapply H0; eauto.
+      subst; auto.
   - (* coinductive halting tau *) use_simpobs. rewrite H. rewrite interp_state_tau.
     pclearbot. pfold. constructor 12; auto.
   - (* coinductive halting vis *)
     use_simpobs. rewrite H. rewrite interp_state_vis.
-    specialize (Hhandler _ e1). inversion Hhandler; try contradiction.
-    specialize (FINCHECK s). induction FINCHECK.
-    + inversion SIZECHECK. contradiction.
-    + rewrite bind_tau. pstep. constructor 12; auto.
-    + rewrite bind_vis. pstep. constructor 14; auto.
+    specialize (Hhandler _ e1). inversion Hhandler; try contradiction; try contra_size.
+    + red in FINCHECK. inv SIZECHECK0. assert (RS s s). admit.  specialize (FINCHECK s s H2).
+      cbn in *. remember (handler _ e1 s) as tspin. clear Heqtspin. clear CIH Heq.
+      generalize dependent tspin. pcofix CIH. intros. punfold FINCHECK.
+      red in FINCHECK. cbn in *. remember (TauF ITree.spin) as ot. remember (observe tspin) as ots.
+      hinduction FINCHECK before r; intros; subst; try discriminate.
+      * use_simpobs. rewrite Heqots. rewrite bind_tau. pfold. constructor 12; auto.
+        right. eapply CIH; eauto. pclearbot. injection Heqot; intros; subst. auto.
+      * use_simpobs. rewrite Heqots. rewrite bind_tau. pstep; constructor; auto.
+        pstep_reverse.
+      * injection Heqot; intros; subst. eapply IHFINCHECK; eauto.
+      * use_simpobs. rewrite Heqots. rewrite bind_vis. pfold. constructor 14; auto.
+        right. pclearbot. eapply CIH; eauto. injection Heqot; intros; subst. apply H3.
+      * use_simpobs. rewrite Heqots. rewrite bind_vis. pfold. red. cbn.
+        assert (VisF e' k' = observe (Vis e' k')). auto. rewrite H5.
+        unpriv_ind. pstep_reverse.
+      * use_simpobs. rewrite Heqots. rewrite bind_vis. pclearbot. pfold. red. cbn. unpriv_halt.
+        contra_size.
   - (* coinductive halting vis *)
     use_simpobs. rewrite H. rewrite interp_state_vis.
-    specialize (Hhandler _ e1). inversion Hhandler; try contradiction.
-    specialize (FINCHECK s). induction FINCHECK.
-    + rewrite bind_ret_l. pstep. constructor 12; auto.
-    + rewrite bind_tau. pstep. constructor 12; auto.
-    + rewrite bind_vis. pstep. constructor 14; auto.
-Qed.
+    specialize (Hhandler _ e1). inversion Hhandler; try contradiction; try contra_size.
+    + red in FINCHECK. inv SIZECHECK0. assert (RS s s). admit.  specialize (FINCHECK a s s H0).
+      remember (handler _ e1) as m. clear Heqm. punfold FINCHECK.
+      red in FINCHECK. cbn in *. remember (observe (m s)) as oms. remember (RetF (s,a)) as oRet.
+      hinduction FINCHECK before r; intros; subst; try contradiction; try discriminate.
+      * use_simpobs. rewrite Heqoms. rewrite bind_ret_l. pstep. constructor 12; auto.
+      * use_simpobs. rewrite Heqoms. rewrite bind_tau. pstep; constructor; auto.
+        pstep_reverse. remember (fun s : S => t1) as m'.  assert (t1 = m' s). subst; auto.
+        rewrite H2. eapply IHFINCHECK; eauto. subst; auto.
+      * use_simpobs. rewrite Heqoms. rewrite bind_vis. pstep. constructor 14; auto.
+        left. remember (fun s : S => k1 a0) as m'. assert (k1 a0 = m' s). subst; auto. rewrite H4. eapply H0; eauto.
+        subst; auto.
+    + red in FINCHECK. inv SIZECHECK0. assert (RS s s). admit.  specialize (FINCHECK s s H2).
+      cbn in *. remember (handler _ e1 s) as tspin. clear Heqtspin. clear CIH Heq.
+      generalize dependent tspin. pcofix CIH. intros. punfold FINCHECK.
+      red in FINCHECK. cbn in *. remember (TauF ITree.spin) as ot. remember (observe tspin) as ots.
+      hinduction FINCHECK before r; intros; subst; try discriminate.
+      * use_simpobs. rewrite Heqots. rewrite bind_tau. pfold. constructor 12; auto.
+        right. eapply CIH; eauto. pclearbot. injection Heqot; intros; subst. auto.
+      * use_simpobs. rewrite Heqots. rewrite bind_tau. pstep; constructor; auto.
+        pstep_reverse.
+      * injection Heqot; intros; subst. eapply IHFINCHECK; eauto.
+      * use_simpobs. rewrite Heqots. rewrite bind_vis. pfold. constructor 14; auto.
+        right. pclearbot. eapply CIH; eauto. injection Heqot; intros; subst. 
+        apply H3.
+      * use_simpobs. rewrite Heqots. rewrite bind_vis. pfold. red. cbn.
+        assert (VisF e' k' = observe (Vis e' k')). auto. rewrite H5. unpriv_ind.
+        pstep_reverse.
+      * use_simpobs. rewrite Heqots. rewrite bind_vis. pfold. pclearbot. red. cbn. unpriv_halt. contra_size.
+Admitted.
+  
+
 
 (* I believe that this is a sound reasoning principle,
    however it looks like the proof could get a little hairy,
@@ -362,54 +597,139 @@ Proof.
     pfold. constructor. right. eapply CIH; eauto. apply H.
   - pclearbot. rewrite Heqot1. rewrite Heqot2.
     rewrite interp_state_tau. rewrite interp_state_vis.
-    specialize (Hhandler A e). inv Hhandler; try contradiction.
-    specialize (FINCHECK s1). induction FINCHECK.
-    + rewrite bind_ret_l. pstep. constructor. right.
-      apply CIH. apply H. etransitivity; [symmetry |]; eauto.
-    + rewrite bind_tau. pstep. constructor 3; auto. pstep_reverse.
-    + rewrite bind_vis. pstep. constructor 9; auto. intros. pstep_reverse.
+    specialize (Hhandler A e). inv Hhandler; try contradiction; try contra_size.
+    red in FINCHECK. inv SIZECHECK0. specialize (FINCHECK a s1 s2 Hs).
+    cbn in FINCHECK. remember (handler A e) as m. clear Heqm.
+    punfold FINCHECK. red in FINCHECK. remember (observe (m s1)) as oms1.
+    remember (observe (Ret (s2, a)) ) as oret.
+    hinduction FINCHECK before r; intros; subst; try discriminate.
+    * injection Heqoret; intros; subst. use_simpobs. rewrite Heqoms1. rewrite bind_ret_l.
+      pfold. constructor. right. destruct H. cbn in *. eapply CIH; eauto.
+      apply H0.
+    * use_simpobs. rewrite Heqoms1. rewrite bind_tau. pstep. constructor 3; auto.
+      pstep_reverse. remember (fun s : S => t1) as m'. assert (t1 = m' s1). subst; auto.
+      rewrite H0. eapply IHFINCHECK; eauto. subst; auto.
+    * use_simpobs. rewrite Heqoms1. rewrite bind_vis.
+      pfold. red. cbn. setoid_rewrite itree_eta' at 3. unpriv_ind.
+      pstep_reverse. remember (fun s : S => k1 a0) as m'. assert (k1 a0 = m' s1). subst; auto.
+      rewrite H2. eapply H0; eauto. subst; auto.
   - pclearbot. rewrite Heqot1. rewrite Heqot2.
     rewrite interp_state_tau. rewrite interp_state_vis.
-    specialize (Hhandler A e). inv Hhandler; try contradiction.
-    specialize (FINCHECK s2). induction FINCHECK.
-    + rewrite bind_ret_l. pstep. constructor. right.
-      apply CIH. apply H. etransitivity; eauto.
-    + rewrite bind_tau. pstep. constructor 4; auto. pstep_reverse.
-    + rewrite bind_vis. pstep. constructor 10; auto. intros. pstep_reverse.
-  - pclearbot. rewrite Heqot1. rewrite Heqot2. repeat rewrite interp_state_vis.
+    specialize (Hhandler A e). inv Hhandler; try contradiction; try contra_size.
+    red in FINCHECK. inv SIZECHECK0. assert (RS s2 s1). symmetry. auto. 
+    specialize (FINCHECK a s2 s1 H0).
+    cbn in FINCHECK. remember (handler A e) as m. clear Heqm.
+    punfold FINCHECK. red in FINCHECK. remember (observe (m s2)) as oms2.
+    remember (observe (Ret (s1, a)) ) as oret.
+    hinduction FINCHECK before r; intros; subst; try discriminate.
+    * injection Heqoret; intros; subst. use_simpobs. rewrite Heqoms2. rewrite bind_ret_l.
+      pfold. constructor. right. destruct H. cbn in *. eapply CIH; eauto.
+      apply H0. symmetry. auto.
+    * use_simpobs. rewrite Heqoms2. rewrite bind_tau. pstep. constructor 4; auto.
+      pstep_reverse. remember (fun s : S => t1) as m'. assert (t1 = m' s2). subst; auto.
+      rewrite H1. eapply IHFINCHECK; eauto. subst; auto.
+    * use_simpobs. rewrite Heqoms2. rewrite bind_vis.
+      pfold. red. cbn. setoid_rewrite itree_eta' at 1. unpriv_ind.
+      pstep_reverse. remember (fun s : S => k1 a0) as m'. assert (k1 a0 = m' s1). subst; auto.
+      rewrite H3. eapply H0; eauto. subst; auto. etransitivity; eauto. subst; auto.
+      etransitivity; eauto.
+  - pclearbot. rewrite Heqot1. rewrite Heqot2.
+    do 2  rewrite interp_state_vis.
     specialize (Hhandler _ e1) as He1. specialize (Hhandler _ e2) as He2.
-    inv He1; inv He2; try contradiction.
-    eapply secure_eqit_bind' with (RR := product_rel RS (fun _ _ => True)).
+    inv He1; inv He2; try contradiction; try contra_size.
+    eapply secure_eqit_bind' with (RR := product_rel RS (fun _ _ => True)); try contra_size.
     + intros [] [] ?. pstep. constructor. right.
       apply CIH. apply H. simpl. apply H0.
-    + specialize (FINCHECK s1). specialize (FINCHECK0 s2).
-      induction FINCHECK.
-      * induction FINCHECK0.
-        -- simpl. pstep. constructor. split; auto. simpl.
-           transitivity s2; eauto. etransitivity; [symmetry |]; eauto.
-        -- pstep. constructor; auto. pstep_reverse.
-        -- pstep. constructor; auto. intros. pstep_reverse. apply H2.
-      * pstep. constructor; auto. pstep_reverse.
-      * pstep. constructor; auto. intros. pstep_reverse. apply H1.
+    + inv SIZECHECK. inv SIZECHECK0. do 2 red in FINCHECK. do 2 red in FINCHECK0.
+      specialize (FINCHECK a s1 s2 Hs). assert (Hs' : RS s2 s1).
+      symmetry; auto.
+      specialize (FINCHECK0 a0 s2 s1 Hs').
+      apply eqit_secure_sym in FINCHECK0.
+      eapply eqit_secure_RR_imp with (RR1 := rcompose (product_rel RS top2) 
+                                                      (flip (product_rel RS top2)) ).
+      {
+        intros [?s ?a] [?s ?b] Hcom. inv Hcom.
+        destruct REL1. destruct REL2. cbn in *. destruct r2. cbn in *.
+        split; try constructor. cbn. etransitivity; eauto. symmetry. auto.
+      }
+      eapply eqit_secure_trans; try apply FINCHECK0. eauto.
+      assert (eqit_secure Label priv2 (product_rel RS top2) true true l 
+                (Ret(s2, a)) (Ret(s1,a0))).
+      { pfold. constructor. constructor. auto. constructor. }
+      eapply eqit_secure_RR_imp; try eapply eqit_secure_trans; eauto.
+      intros. inv PR. 
+      destruct x0; destruct x1; destruct r2. split; try constructor.
+      cbn in *. destruct REL1. destruct REL2. cbn in *. etransitivity; eauto.
   - rewrite Heqot1. rewrite interp_state_vis. specialize (Hhandler _ e).
-    inv Hhandler; try contradiction.
-    specialize (FINCHECK s1). induction FINCHECK.
-    + rewrite bind_ret_l. pstep. constructor; auto. pstep_reverse.
-      eapply H0; eauto. simpl. etransitivity; [symmetry |]; eauto.
-    + rewrite bind_tau. pstep. constructor 3; auto. pstep_reverse.
-    + rewrite bind_vis. pstep. constructor 9; auto. intros. pstep_reverse.
+    inv Hhandler; try contradiction; try contra_size. inv SIZECHECK0.
+    specialize (FINCHECK a s1 s2 Hs). 
+    cbn in FINCHECK. remember (handler A e) as m. clear Heqm.
+    punfold FINCHECK. red in FINCHECK. remember (observe (m s1)) as oms1.
+    remember (observe (Ret (s2, a)) ) as oret.
+    hinduction FINCHECK before r; intros; subst; try discriminate.
+    * injection Heqoret; intros; subst. use_simpobs. rewrite Heqoms1. rewrite bind_ret_l.
+      pfold. constructor; auto. pstep_reverse. eapply H1; eauto.
+      destruct H. auto.
+    * use_simpobs. rewrite Heqoms1. rewrite bind_tau. pstep. constructor 3; auto.
+      pstep_reverse. remember (fun s : S => t1) as m'. assert (t1 = m' s1). subst; auto.
+      rewrite H1. eapply IHFINCHECK; eauto. subst; auto.
+    * use_simpobs. rewrite Heqoms1. rewrite bind_vis.
+      pfold. red. cbn. setoid_rewrite itree_eta' at 1. unpriv_ind.
+      pstep_reverse. remember (fun s : S => k1 a0) as m'. assert (k1 a0 = m' s1). subst; auto.
+      rewrite H3. cbn. eapply H0; eauto. subst; auto.
   - rewrite Heqot2. rewrite interp_state_vis. specialize (Hhandler _ e).
-    inv Hhandler; try contradiction.
-    specialize (FINCHECK s2). induction FINCHECK.
-    + rewrite bind_ret_l. pstep. constructor 4; auto. pstep_reverse.
-      eapply H0; eauto. simpl. etransitivity; eauto.
-    + rewrite bind_tau. pstep. constructor 4; auto. pstep_reverse.
-    + rewrite bind_vis. pstep. constructor 10; auto. intros. pstep_reverse.
+    inv Hhandler; try contradiction; try contra_size. inv SIZECHECK0.
+    symmetry in Hs.
+    specialize (FINCHECK a s2 s1 Hs). 
+    cbn in FINCHECK. remember (handler A e) as m. clear Heqm.
+    punfold FINCHECK. red in FINCHECK. remember (observe (m s2)) as oms2.
+    remember (observe (Ret (s1, a)) ) as oret.
+    hinduction FINCHECK before r; intros; subst; try discriminate.
+    * injection Heqoret; intros; subst. use_simpobs. rewrite Heqoms2. rewrite bind_ret_l.
+      pfold. constructor; auto. pstep_reverse. eapply H1; eauto.
+      destruct H. auto. symmetry. auto.
+    * use_simpobs. rewrite Heqoms2. rewrite bind_tau. pstep. constructor 4; auto.
+      pstep_reverse. remember (fun s : S => t1) as m'. assert (t1 = m' s1). subst; auto.
+      rewrite H1. eapply IHFINCHECK; eauto. subst; auto. etransitivity; eauto.
+      symmetry. auto. subst; auto.
+    * use_simpobs. rewrite Heqoms2. rewrite bind_vis.
+      pfold. red. cbn. timeout 10 setoid_rewrite itree_eta' at 2. unpriv_ind.
+      pstep_reverse. remember (fun s : S => k1 a0) as m'. assert (k1 a0 = m' s1). subst; auto.
+      rewrite H3. cbn. eapply H0; eauto. subst; auto.
+      etransitivity; eauto. symmetry; auto. subst; auto.
   - pclearbot.
     rewrite Heqot1. rewrite interp_state_vis.
     rewrite Heqot2. rewrite interp_state_tau.
     pose proof Hhandler as Hhandler'.
-    specialize (Hhandler' _ e). inv Hhandler'; try contradiction.
+    specialize (Hhandler' _ e). inv Hhandler'; try contradiction; try contra_size.
+    specialize (FINCHECK s1 s2 Hs).
+    
+    admit.
+  - rewrite Heqot2. rewrite Heqot1. pclearbot.
+    rewrite interp_state_vis. rewrite interp_state_tau. admit.
+  - pclearbot. admit.
+  -
+    remember (handler A e s1) as tspin. clear Heqtspin. pfold. constructor; auto.
+    pstep_reverse.
+    generalize dependent tspin. clear Heqot2. generalize dependent t2. clear CIH. pcofix CIH. intros. punfold FINCHECK.
+    red in FINCHECK. cbn in *. remember (TauF ITree.spin) as ot. remember (observe tspin) as ots.
+    hinduction FINCHECK before r; intros; subst; try discriminate.
+    * use_simpobs. rewrite Heqots. rewrite bind_tau.
+      pinversion H0; try inv Heqot; ITrace.inj_existT; subst; try contra_size.
+      ++ use_simpobs. rewrite H1. rewrite interp_state_tau.
+         pfold. constructor; eauto.
+      ++ use_simpobs. rewrite H5. rewrite interp_state_vis.
+      constructor. auto.
+      pclearbot. eapply CIH; eauto.
+      right. eapply CIH; eauto. pclearbot. injection Heqot; intros; subst. auto.
+    * use_simpobs. rewrite Heqots. rewrite bind_tau. pstep; constructor; auto.
+      pstep_reverse.
+    * injection Heqot; intros; subst. eapply IHFINCHECK; eauto.
+    * use_simpobs. rewrite Heqots. rewrite bind_vis. pfold. constructor 13; auto.
+      right. pclearbot. eapply CIH; eauto. injection Heqot; intros; subst. apply H2.
+    * use_simpobs. rewrite Heqots. rewrite bind_vis. pfold. red. cbn. rewrite itree_eta' at 1. unpriv_ind. 
+        pstep_reverse.
+      * use_simpobs. rewrite Heqots. rewrite bind_vis. pfold. pclearbot. red. cbn. unpriv_halt. contra_size.
     specialize (FINCHECK s1). induction FINCHECK.
     + inversion SIZECHECK. contradiction.
     + rewrite bind_tau. pstep. constructor 3; auto. pstep_reverse.
